Simplify semantics of succ.

Cslib/Computability/Machines/MultiTapeTuring/SuccRoutine.lean
@@ -25,54 +25,22 @@ def succ₀ : MultiTapeTM 1 (WithSep OneTwo) where
   M _ syms := sorry
 
 @[simp]
-lemma succ₀_eval_list {n : ℕ} {ls : List (List OneTwo)} :
-  succ₀.eval_list [(dya n) :: ls].get = .some [(dya n.succ) :: ls].get := by
+lemma succ₀_eval_list {tapes : Fin 1 → List (List OneTwo)} :
+  succ₀.eval_list tapes = .some (Function.update tapes 0
+    ((dya (dya_inv ((tapes 0).headD [])).succ) :: (tapes 0).tail)) := by
   sorry
 
 /--
 A Turing machine that increments the head of tape `i` by one (in dyadic encoding).
 Pushes zero if the tape is empty. -/
 public def succ {k : ℕ} (i : Fin k) : MultiTapeTM k (WithSep OneTwo) :=
-  succ₀.with_tapes (fun _ => i) (by intro x y; grind)
-
-/--
-The function computed by `succ`.
--/
-public def succ_f {k : ℕ}
-  (i : Fin k)
-  (tapes : Fin k → List (List OneTwo)) : Fin k → List (List OneTwo) :=
-  if h_ne : tapes i ≠ [] then
-    Function.update tapes i ((dya ((dya_inv ((tapes i).head h_ne)).succ)) :: (tapes i).tail)
-  else
-    tapes
-
-@[simp]
-public lemma succ_f_neq {k : ℕ}
-  (i : Fin k)
-  (tapes : Fin k → List (List OneTwo))
-  (h_ne : tapes i ≠ []) :
-  succ_f i tapes = Function.update tapes i
-    ((dya ((dya_inv ((tapes i).head h_ne)).succ)) :: (tapes i).tail) := by
-  simp [succ_f, h_ne]
-
-@[simp]
-public lemma succ_f_empty {k : ℕ}
-  (i : Fin k)
-  (tapes : Fin k → List (List OneTwo))
-  (h_empty : tapes i = []) :
-  succ_f i tapes = tapes := by
-  simp [succ_f, h_empty]
-
-@[simp]
-public theorem succ_computes {k : ℕ} {i : Fin k} :
-  (succ i).computes (succ_f i) := by
-  sorry
+  succ₀.with_tapes [i].get (by intro x y; grind)
 
 @[simp]
 public theorem succ_eval_list {k : ℕ} {i : Fin k} {tapes : Fin k → List (List OneTwo)} :
-  (succ i).eval_list tapes = .some (succ_f i tapes) := by
-  -- TOOD why does simp not find it?
-  simp [MultiTapeTM.eval_of_computes succ_computes]
+  (succ i).eval_list tapes = .some (Function.update tapes i
+    ((dya (dya_inv ((tapes i).headD [])).succ) :: (tapes i).tail)) := by
+  simpa [succ] using apply_updates_function_update (by intro x y; grind)
 
 lemma succ₀_evalWithStats_list {n : ℕ} {ls : List (List OneTwo)} :
   succ₀.evalWithStats_list [(dya n) :: ls].get =
